adding proof attempt linking weak step sequence to tradce formulas

Weak_Traces.thy
@@ -9,6 +9,45 @@ inductive
   "is_trace_formula (Internal \<chi>)" if "is_trace_formula_conjunction \<chi>" |
   "is_trace_formula_conjunction (Obs \<alpha> \<phi>)" if "is_trace_formula \<phi>"
 
+primrec \<phi>_wtraces :: "('act, 'i) hml_srbb \<Rightarrow> 'act list set"
+  and \<chi>_wtraces :: "('act, 'i) hml_srbb_conjunction \<Rightarrow> 'act list set"
+  and \<psi>_wtraces :: "('act, 'i) hml_srbb_conjunct \<Rightarrow> 'act list set" where
+  "\<phi>_wtraces TT = {[]}" |
+  "\<phi>_wtraces (Internal \<chi>) = \<chi>_wtraces \<chi>" |
+  "\<phi>_wtraces (ImmConj I \<psi>s) = \<Union>((\<psi>_wtraces \<circ> \<psi>s) ` I)" |
+
+  "\<chi>_wtraces (Obs \<alpha> \<phi>) = (\<lambda>tr. \<alpha> # tr) ` (\<phi>_wtraces \<phi>)" |
+  "\<chi>_wtraces (Conj I \<psi>s) = \<Union>((\<psi>_wtraces \<circ> \<psi>s) ` I)" |
+  "\<chi>_wtraces (StableConj I \<psi>s) = \<Union>((\<psi>_wtraces \<circ> \<psi>s) ` I)" |
+  "\<chi>_wtraces (BranchConj \<alpha> \<phi> I \<psi>s) = (\<lambda>tr. \<alpha> # tr) ` (\<phi>_wtraces \<phi>) \<union> \<Union>((\<psi>_wtraces \<circ> \<psi>s) ` I)" |
+
+  "\<psi>_wtraces (Pos \<chi>) = \<chi>_wtraces \<chi>" |
+  "\<psi>_wtraces (Neg \<chi>) = \<chi>_wtraces \<chi>" \<comment> \<open> This case is problematic! Actually, I want to reject all those traces... \<close>
+
+lemma 
+  fixes \<phi> :: "('act, 'i) hml_srbb"
+  fixes \<chi> :: "('act, 'i) hml_srbb_conjunction"
+  shows "(is_trace_formula \<phi> \<longrightarrow> (\<exists>tr. \<phi>_wtraces \<phi> = {tr}))
+       \<and> (is_trace_formula_conjunction \<chi> \<longrightarrow> (\<exists>tr. \<chi>_wtraces \<chi> = {tr}))"
+  apply (induct rule: is_trace_formula_is_trace_formula_conjunction.induct)
+  by fastforce+
+
+fun wtrace_to_\<phi> :: "'act list \<Rightarrow> ('act, 'i) hml_srbb"
+  and wtrace_to_\<chi> :: "'act list \<Rightarrow> ('act, 'i) hml_srbb_conjunction"
+  and wtrace_to_\<psi> :: "'act list \<Rightarrow> ('act, 'i) hml_srbb_conjunct" where
+  "wtrace_to_\<phi> [] = TT" |
+  "wtrace_to_\<phi> tr = (Internal (wtrace_to_\<chi> tr))" |
+
+  "wtrace_to_\<chi> [] = (Conj {} (\<lambda>_. undefined))" | \<comment> \<open> Should never happen\<close>
+  "wtrace_to_\<chi> (\<alpha> # tr) = (Obs \<alpha> (wtrace_to_\<phi> tr))" |
+
+  "wtrace_to_\<psi> tr = Pos (wtrace_to_\<chi> tr)" \<comment> \<open>Should never happen\<close>
+
+lemma "is_trace_formula (wtrace_to_\<phi> trace)"
+  apply (induct trace)
+  using is_trace_formula_is_trace_formula_conjunction.intros
+  by fastforce+
+
 lemma trace_formula_to_expressiveness:
   fixes \<phi> :: "('act, 'i) hml_srbb"
   fixes \<chi> :: "('act, 'i) hml_srbb_conjunction"
@@ -47,6 +86,87 @@ lemma
 
 lemma "(p \<lesssim>WT q) = (p \<preceq> (E \<infinity> 0 0 0 0 0 0 0) q)"
   sorry
+
+
+lemma "p \<Zsurj>\<mapsto>\<Zsurj>$ t p' \<Longrightarrow> \<exists>\<phi>. is_trace_formula \<phi> \<and> \<phi> \<Turnstile>SRBB p \<and> wtrace_to_\<phi> t = \<phi>"
+proof (induction t arbitrary: p)
+  case Nil
+  then show ?case 
+    using is_trace_formula_is_trace_formula_conjunction.intros(1) by force
+next
+  case (Cons \<alpha> tail)
+
+  assume IH: "\<And>p1. p1 \<Zsurj>\<mapsto>\<Zsurj>$ tail p' \<Longrightarrow> \<exists>\<phi>. is_trace_formula \<phi> \<and> \<phi> \<Turnstile>SRBB p1 \<and> wtrace_to_\<phi> tail = \<phi>"
+    and "p \<Zsurj>\<mapsto>\<Zsurj>$ (\<alpha> # tail) p'"
+  hence "\<exists>m. p \<Zsurj>\<mapsto>\<Zsurj> \<alpha> m \<and> m \<Zsurj>\<mapsto>\<Zsurj>$ tail p'" 
+    using weak_step_sequence.cases by fastforce
+  then obtain m where "p \<Zsurj>\<mapsto>\<Zsurj> \<alpha> m" and "m \<Zsurj>\<mapsto>\<Zsurj>$ tail p'" 
+    by blast
+  then have "\<exists>\<phi>. is_trace_formula \<phi> \<and> \<phi> \<Turnstile>SRBB m \<and> wtrace_to_\<phi> tail = \<phi>" using IH
+    by blast
+  then obtain \<phi>_tail where "is_trace_formula \<phi>_tail"
+                  and "\<phi>_tail \<Turnstile>SRBB m"
+                  and "wtrace_to_\<phi> tail = \<phi>_tail" by blast
+  define \<phi> where "\<phi> \<equiv> (Internal (Obs \<alpha> \<phi>_tail))"
+
+  have "is_trace_formula \<phi>"
+    using \<open>is_trace_formula \<phi>_tail\<close>
+      and is_trace_formula_is_trace_formula_conjunction.intros
+      and \<phi>_def
+    by force
+
+  have "wtrace_to_\<phi> (\<alpha> # tail) = \<phi>"
+    using \<open>wtrace_to_\<phi> tail = \<phi>_tail\<close>
+      and \<phi>_def by force
+
+  have "\<phi> \<Turnstile>SRBB p"
+    using \<open>p \<Zsurj>\<mapsto>\<Zsurj> \<alpha> m\<close>
+      and \<open>\<phi>_tail \<Turnstile>SRBB m\<close>
+    unfolding \<phi>_def
+      and hml_srbb_models.simps
+      and hml_srbb_to_hml.simps
+    unfolding hml_models.simps
+      and hml_srbb_conjunction_to_hml.simps
+  proof -
+    assume "p \<Zsurj>\<mapsto>\<Zsurj> \<alpha> m"
+       and "hml_srbb_to_hml \<phi>_tail \<Turnstile> m"
+
+    show "\<exists>p'. p \<Zsurj> p' \<and> (\<exists>p'a. p' \<mapsto> \<alpha> p'a \<and> ((hml_srbb_to_hml \<phi>_tail) \<Turnstile> p'a))"
+    proof (cases \<open>\<alpha> = \<tau>\<close>)
+      case True
+      hence "\<alpha> = \<tau>".
+
+      from \<open>p \<Zsurj>\<mapsto>\<Zsurj> \<alpha> m\<close> and \<open>\<alpha> = \<tau>\<close>
+      have "p \<Zsurj> m" 
+        using weak_step_def by auto
+
+      then show ?thesis sorry
+    next
+      case False
+      hence "\<alpha> \<noteq> \<tau>".
+
+      from \<open>p \<Zsurj>\<mapsto>\<Zsurj> \<alpha> m\<close> and \<open>\<alpha> \<noteq> \<tau>\<close>
+      have "\<exists>p1 p2. p \<Zsurj> p1 \<and> p1 \<mapsto> \<alpha> p2 \<and> p2 \<Zsurj> m"
+        using weak_step_def by auto
+      then obtain ml and mr where "p \<Zsurj> ml" and "ml \<mapsto> \<alpha> mr" and "mr \<Zsurj> m"
+        by blast
+
+      from \<open>hml_srbb_to_hml \<phi>_tail \<Turnstile> m\<close>
+       and \<open>mr \<Zsurj> m\<close>
+       and \<open>is_trace_formula \<phi>_tail\<close>
+      have "hml_srbb_to_hml \<phi>_tail \<Turnstile> mr" sorry
+
+      then show ?thesis 
+        using \<open>ml \<mapsto> \<alpha> mr\<close> \<open>p \<Zsurj> ml\<close> by blast
+    qed
+  qed
+
+  then show ?case
+    using \<open>is_trace_formula \<phi>\<close>
+      and \<open>\<phi> \<Turnstile>SRBB p\<close>
+      and \<open>wtrace_to_\<phi> (\<alpha> # tail) = \<phi>\<close>
+    by blast
+qed
 
 end
 
